\appendix
\renewcommand{\thechapter}{A}
\chapter{Calculation results of field-field correlation function}
\label{appendix:CF}

For field-field correlation function, in the free propagation case, the original calculation results are:

\begin{align}
\frac{C_E({\bf r}_1,{\bf r}_2;z)}{E_0^2} =& \left[\frac{w}{w(z)}\right]^2 \exp(-ik_0\frac{{\bf r}_1^2 - {\bf r}_2^2}{2 R(z)})\\
&\times \exp(-\frac{{\bf r}_1^2 + {\bf r}_2^2}{w(z)^2})\exp(-\frac{|{\bf r}_1-{\bf r}_2|^2}{\sigma(z)^2}) \nonumber 
\end{align}

\begin{equation}
    \begin{cases}
    %&{\bf \bar{r}}=({\bf r_1}+{\bf r_2})/2\\
    &1/R(z) = 1/z - k_0^2w^2/8Az^3\\
    &1/\sigma^2(z)=k_0^2w^2/8z^2 - k_0^4w^4/64Az^4 - k_0^2/16Az^2\\
    &1/w^2(z) = k_0^2/8Az^2\\
    &A = 1/2w^2 + 1/\sigma^2 + k_0^2w^2/8z^2
    \end{cases}
\end{equation}

With a lens, 
\begin{align}
\frac{C_E({\bf r}_1,{\bf r}_2;z)}{E_0^2} =& \frac{k_0^2w^2}{4z^2D} \exp\left[-i\left(\frac{k_0}{2z} + \frac{z_L^2AB}{2Dz^2}\right)({\bf r}_1^2 - {\bf r}_2^2)\right]\\
&\times \exp\left[-\frac{k_0^2({\bf r}_1^2 + {\bf r}_2^2)}{4z^2D}\right]\exp\left[-\left( \frac{z_L^2A}{2z^2} -\frac{z_L^4A^2B^2}{2k_0^2z^2D} - \frac{k_0^2}{8z^2D}\right)|{\bf r}_1-{\bf r}_2|^2\right] \nonumber 
\end{align}
where,
\begin{equation}
    \begin{cases}
    &A = 1/2w^2 + 1/\sigma^2 + k_0^2w^2/8z_L^2\\
    &B = \frac{k_0^3w^2}{8z_L^3A} - k_0(1/z+1/z_L-1/f)\\
    &C = \frac{k_0^2w^2}{8z_L^2} - \frac{k_0^4w^4}{64z_L^4A}\\
    &D = \frac{z_L^2AB^2}{k_0^2} + C\\
    \end{cases}
\end{equation}